Examples/SignedDH/SecurityTheorems.lean
@@ -1,49 +1,131 @@
-module
+-- module -- no module to use `#print axioms`
 
-public import DY.Step
+import DY.Step
 import DY.Step.Utils
-public import Examples.SignedDH.Specification
-public import Examples.SignedDH.Proof
-import all Examples.SignedDH.Proof
+import Examples.SignedDH.Specification
+import Examples.SignedDH.Proof
 
 namespace DY.Example.SignedDH
+
+def honest: Traceful Unit := do
+  let (_, tsPk, tsSk) ← LongTermKeys.generateKeyPair "SignedDH" "Bob" -- 4
+  let (tsClientSt, tsMsgClient) ← client_initiate "Alice" -- 4
+  let (_tsServerSt, tsMsgServer) ← server_receive "Bob" tsSk tsMsgClient -- 5
+  let _ ← client_finish "Alice" "Bob" tsPk tsMsgServer tsClientSt -- 2
+
+theorem honest_PreservesReachability
+  : honest.PreservesReachability reachability
+:= by
+  unfold Traceful.PreservesReachability
+  intro tr h_tr
+  unfold honest
+  apply Traceful.PreservesReachabilityFrom_bind
+  · assumption
+  · apply Traceful.PreservesReachabilityFrom_base (LongTermKeys.reachability "SignedDH")
+    simp
+  intro ⟨ _, tsPk, tsSk ⟩ tr h_tr h_le
+  dsimp only
+  apply Traceful.PreservesReachabilityFrom_bind
+  · assumption
+  · apply Traceful.PreservesReachabilityFrom_base (.make (fun me => client_initiate me))
+    simp
+  intro ⟨ tsClientSt, tsMsgClient ⟩ tr h_tr h_le
+  dsimp only
+  apply Traceful.PreservesReachabilityFrom_bind
+  · assumption
+  · apply Traceful.PreservesReachabilityFrom_base (.make (fun (me, sk_ts, msg_ts) => server_receive me sk_ts msg_ts)) _ ("Bob", tsSk, tsMsgClient)
+    simp
+  intro ⟨ _, tsMsgServer ⟩ tr h_tr h_le
+  dsimp only
+  apply Traceful.PreservesReachabilityFrom_bind
+  · assumption
+  · apply Traceful.PreservesReachabilityFrom_base (.make (fun (me, server, pk_ts, msg_ts, sid) => client_finish me server pk_ts msg_ts sid)) _ ("Alice", "Bob", tsPk, tsMsgServer, tsClientSt)
+    simp
+  intro _ tr h_tr h_le
+  apply Traceful.PreservesReachabilityFrom_pure
+
+theorem sanity_check:
+  ∃ tr: ExecTrace,
+    tr.Reachable reachability ∧
+    ∃ t1 t2 xPk yPk k,
+      t1 < t2 ∧
+      tr.EventLoggedAt (SignedDHEvent.ServerFinishEvent "Bob" xPk yPk k) t1 ∧
+      tr.EventLoggedAt (SignedDHEvent.ClientFinishEvent "Alice" "Bob" xPk yPk k) t2
+:= by
+  exists (honest.run (Trace.nil)).snd
+  apply And.intro
+  · exact honest_PreservesReachability Trace.nil (Trace.ReachableFrom.Base)
+  exists 10
+  exists 13
+  simp only [DY.Trace.EventLoggedAt_eq_getEventAt]
+  let witness :=
+    match (Trace.getEventAt SignedDHEvent 10 (honest.run Trace.nil).snd.val) with
+    | some (SignedDHEvent.ServerFinishEvent _ xPk yPk k) => (xPk, yPk, k)
+    | _ => (Comparse.BytesLike.empty, Comparse.BytesLike.empty, Comparse.BytesLike.empty)
+  exists witness.fst
+  exists witness.snd.fst
+  exists witness.snd.snd
+  native_decide
+
+/--
+info: 'DY.Example.SignedDH.sanity_check' depends on axioms: [propext,
+ Classical.choice,
+ Quot.sound,
+ sanity_check._native.native_decide.ax_1_5]
+-/
+#guard_msgs in
+#print axioms sanity_check
 
 theorem client_auth
   (client server: Participant)
   (xPk yPk k: Bytes)
   (time: Nat)
-  (tr: ProofTrace):
-  tr.Invariant → -- reachable
-  tr.erase.EventLoggedAt (SignedDHEvent.ClientFinishEvent client server xPk yPk k) time →
-  (
-    let tr_before := tr.prefix time
-    tr_before.erase.EventLogged (SignedDHEvent.ServerFinishEvent server xPk yPk k) ∨
-    (∃ spk, LongTermKeys.LongTermKeyCompromised "SignedDH" server spk tr_before.erase)
-  )
+  : ∀ tr: ExecTrace,
+    tr.Reachable reachability →
+    tr.EventLoggedAt (SignedDHEvent.ClientFinishEvent client server xPk yPk k) time →
+    (
+      let tr_before := tr.prefix time
+      tr_before.EventLogged (SignedDHEvent.ServerFinishEvent server xPk yPk k) ∨
+      (∃ spk, LongTermKeys.LongTermKeyCompromised "SignedDH" server spk tr_before)
+    )
 := by
-  intro h_trinv h_ev
+  apply Trace.apply_Reachable_implies_Invariant
+  intro tr h_trinv h_ev
   have := Trace.EventLoggedAt_imp_EventInv _ _ _ h_trinv h_ev
   simp [ProtocolEvent.EventInv.invariant, LongTermKeys.label] at this
   grind
 
+/--
+info: 'DY.Example.SignedDH.client_auth' depends on axioms: [propext, Classical.choice, Quot.sound]
+-/
+#guard_msgs in
+#print axioms client_auth
+
 theorem client_secrecy
   (client server: Participant)
   (xPk yPk k: Bytes)
-  (tr: ProofTrace):
-  tr.Invariant → -- reachable
-  k.AttackerKnows tr.erase →
-  tr.erase.EventLoggedAt (SignedDHEvent.ClientFinishEvent client server xPk yPk k) time →
-  (
-    let tr_before := tr.prefix time
-    (∃ spk, LongTermKeys.LongTermKeyCompromised "SignedDH" server spk tr_before.erase) ∨
-    ClientEphemeralStateCompromised client xPk tr.erase ∨
-    ServerEphemeralStateCompromised server yPk tr.erase
-  )
-  := by
-    intro h_trinv h_pub h_ev
-    have := Trace.EventLoggedAt_imp_EventInv _ _ _ h_trinv h_ev
-    simp [ProtocolEvent.EventInv.invariant] at this
-    simp_all [client_label, server_label, LongTermKeys.label]
-    grind
+  : ∀ tr: ExecTrace,
+    tr.Reachable reachability →
+    k.AttackerKnows tr →
+    tr.EventLoggedAt (SignedDHEvent.ClientFinishEvent client server xPk yPk k) time →
+    (
+      let tr_before := tr.prefix time
+      (∃ spk, LongTermKeys.LongTermKeyCompromised "SignedDH" server spk tr_before) ∨
+      ClientEphemeralStateCompromised client xPk tr ∨
+      ServerEphemeralStateCompromised server yPk tr
+    )
+:= by
+  apply Trace.apply_Reachable_implies_Invariant
+  intro tr h_trinv h_pub h_ev
+  have := Trace.EventLoggedAt_imp_EventInv _ _ _ h_trinv h_ev
+  simp [ProtocolEvent.EventInv.invariant] at this
+  simp_all [client_label, server_label, LongTermKeys.label]
+  grind
+
+/--
+info: 'DY.Example.SignedDH.client_secrecy' depends on axioms: [propext, Classical.choice, Quot.sound]
+-/
+#guard_msgs in
+#print axioms client_secrecy
 
 end DY.Example.SignedDH
