DY/Trace.lean
@@ -5,4 +5,6 @@ public import DY.Trace.BaseAttackerKnowledge
 public import DY.Trace.Invariant
 public import DY.Trace.BaseAttackerKnowledgeTheorem
 public import DY.Trace.Manipulation
+public import DY.Trace.Reachability
+public import DY.Trace.ReachabilityTheorem
 public meta import DY.Trace.Grind
