DY/Trace/Reachability.lean
@@ -1,0 +1,167 @@
+module
+
+public import DY.Trace.Manipulation
+
+namespace DY
+
+variable [ExecTraceTypes]
+
+public
+structure ReachabilityConfig where
+  Input: Type
+  PreCond: Input → ExecTrace → Prop
+  step: Input → (Output: Type) × Traceful Output
+
+public
+abbrev ReachabilityConfig.make
+  {α β: Type}
+  (step: α → Traceful β)
+  : ReachabilityConfig
+where
+  Input := α
+  PreCond _ _ := True
+  step x := ⟨ _, step x ⟩
+
+@[expose]
+public
+def ReachabilityConfig.combine {α: Type} (configs: α → ReachabilityConfig): ReachabilityConfig where
+  Input := (x: α) × (configs x).Input
+  PreCond := fun ⟨ x, inp ⟩ tr => (configs x).PreCond inp tr
+  step := fun ⟨ x, inp ⟩ => (configs x).step inp
+
+public
+class ReachabilityConfig.HasStep (config1: ReachabilityConfig) (config2: semiOutParam ReachabilityConfig) where
+  inj: config1.Input → config2.Input
+  pf_pre: ∀ input tr, config1.PreCond input tr = config2.PreCond (inj input) tr
+  pf_step: ∀ input, config1.step input = config2.step (inj input)
+
+public
+class ReachabilityConfig.Has (config1 config2: ReachabilityConfig) where
+  inj: config1.Input → config2.Input
+  pf_pre: ∀ input tr, config1.PreCond input tr = config2.PreCond (inj input) tr
+  pf_step (config1 config2): ∀ input, config1.step input = config2.step (inj input)
+
+public
+instance
+  (config: ReachabilityConfig)
+  : ReachabilityConfig.Has config config
+where
+  inj x := x
+  pf_pre input tr := by simp
+  pf_step input := by simp
+
+public
+instance
+  (config1 config2 config3: ReachabilityConfig)
+  [inst12: ReachabilityConfig.HasStep config1 config2]
+  [inst23: ReachabilityConfig.Has config2 config3]
+  : ReachabilityConfig.Has config1 config3
+where
+  inj x := inst23.inj (inst12.inj x)
+  pf_pre input tr := by simp [inst23.pf_pre, inst12.pf_pre]
+  pf_step input := by simp [inst23.pf_step, inst12.pf_step]
+
+public
+instance
+  {α: Type}
+  (configs: α → ReachabilityConfig)
+  (id: α)
+  : ReachabilityConfig.HasStep (configs id) (.combine configs)
+where
+  inj x := ⟨ id, x ⟩
+  pf_pre input tr := by simp [ReachabilityConfig.combine]
+  pf_step input := by simp [ReachabilityConfig.combine]
+
+public
+inductive Trace.ReachableFrom (config: ReachabilityConfig) (trIn: ExecTrace): ExecTrace → Prop where
+  | Base:
+    Trace.ReachableFrom config trIn trIn
+  | Step:
+    {trMid: ExecTrace} →
+    (input: config.Input) →
+    config.PreCond input trMid →
+    Trace.ReachableFrom config trIn trMid →
+    Trace.ReachableFrom config trIn (Traceful.run ((config.step input).snd) trMid).snd
+
+public
+theorem Trace.ReachableFrom_trans
+  (config: ReachabilityConfig)
+  (tr1 tr2 tr3: ExecTrace)
+  : Trace.ReachableFrom config tr1 tr2 →
+    Trace.ReachableFrom config tr2 tr3 →
+    Trace.ReachableFrom config tr1 tr3
+:= by
+  intro h12 h23
+  induction h23
+  · exact h12
+  · rename_i trIn trOut input h_input h_reach1 h_reach2
+    apply Trace.ReachableFrom.Step input <;> grind
+
+public
+def Trace.Reachable (config: ReachabilityConfig) (tr: ExecTrace): Prop :=
+  Trace.ReachableFrom config Trace.nil tr
+
+public
+def Traceful.PreservesReachabilityFrom {a: Type} (config: ReachabilityConfig) (f: Traceful a) (tr: ExecTrace): Prop :=
+    Trace.ReachableFrom config tr (Traceful.run f tr).snd
+
+public
+def Traceful.PreservesReachability {a: Type} (config: ReachabilityConfig) (f: Traceful a): Prop :=
+  ∀ tr,
+    tr.Reachable config →
+    Trace.ReachableFrom config tr (Traceful.run f tr).snd
+
+public
+theorem Traceful.PreservesReachabilityFrom_bind
+  {a b: Type}
+  (config: ReachabilityConfig)
+  (x: Traceful a) (f: a → Traceful b)
+  (tr: ExecTrace)
+  : tr.Reachable config →
+    x.PreservesReachabilityFrom config tr →
+    (∀ x' trMid,
+      trMid.Reachable config →
+      tr ≤ trMid →
+      (f x').PreservesReachabilityFrom config trMid
+    ) →
+    (x >>= f).PreservesReachabilityFrom config tr
+:= by
+  intro h_tr h_x h_next
+  simp_all only [Traceful.PreservesReachabilityFrom, Traceful.run_bind]
+  cases h: (x.run tr).fst
+  · simp_all
+  · refine Trace.ReachableFrom_trans _ _ (x.run tr).snd _ ?_ ?_
+    · grind
+    · rename_i val
+      refine h_next val (x.run tr).snd ?_ ?_
+      · grind [Trace.Reachable, Trace.ReachableFrom_trans]
+      · exact (x.run tr).snd.property
+
+public
+theorem Traceful.PreservesReachabilityFrom_base
+  (subConfig config: ReachabilityConfig)
+  [ReachabilityConfig.Has subConfig config]
+  (input: subConfig.Input)
+  (tr: ExecTrace)
+  : subConfig.PreCond input tr →
+    (subConfig.step input).snd.PreservesReachabilityFrom config tr
+:= by
+  intro h_input
+  dsimp only [Traceful.PreservesReachabilityFrom]
+  rewrite [ReachabilityConfig.Has.pf_step subConfig config]
+  apply Trace.ReachableFrom.Step (ReachabilityConfig.Has.inj input)
+  · grind [ReachabilityConfig.Has.pf_pre]
+  · apply Trace.ReachableFrom.Base
+
+public
+theorem Traceful.PreservesReachabilityFrom_pure
+  {α: Type}
+  (config: ReachabilityConfig)
+  (x: α)
+  (tr: ExecTrace)
+  : (pure x: Traceful α).PreservesReachabilityFrom config tr
+:= by
+  simp only [Traceful.PreservesReachabilityFrom, Traceful.run_pure]
+  apply Trace.ReachableFrom.Base
+
+end DY
